Logic/Modal/Normal/Soundness.lean
@@ -6,10 +6,10 @@ namespace LO.Modal.Normal
 
 open Formula FrameConsequence
 
-variable (α β : Type u) [Inhabited β]
+variable (α β : Type u)[Inhabited β]
 
 lemma Logic.Hilbert.sounds
-  (Λ : Logic α)
+  (Λ : AxiomSet α)
   (f : Frame β) (hf : f ∈ (FrameClass β α Λ))
   {p : Formula α}
   (d : ⊢ᴹ(Λ) p) : (⊧ᴹᶠ[f] p) := by
@@ -23,7 +23,7 @@ lemma Logic.Hilbert.sounds
     | inr hq => exact hqr hq;
 
 lemma Logic.Hilbert.consistent
-  (Λ : Logic α)
+  (Λ : AxiomSet α)
   (hf : ∃ f, f ∈ (FrameClass β α Λ))
   : (⊬ᴹ(Λ)! (⊥ : Formula α)) := by
   by_contra hC; simp at hC;
@@ -34,15 +34,18 @@ lemma Logic.Hilbert.consistent
   existsi tf;
   exact Logic.Hilbert.sounds _ _ Λ tf htf hC.some;
 
-variable {α β : Type u} [Inhabited β] {p : Formula α} (f : Frame β)
+variable {α β : Type u} [Inhabited α] [Inhabited β] {p : Formula α} (f : Frame β)
 
 theorem LogicK.Hilbert.sounds : (⊢ᴹ(𝐊) p) → (⊧ᴹᶠ[f] p) := Logic.Hilbert.sounds _ _ 𝐊 f (def_FrameClass f)
-theorem LogicK.Hilbert.consistency : ⊬ᴹ(𝐊)! (⊥ : Formula α) := Logic.Hilbert.consistent α β 𝐊 (by existsi ((λ _ _ => True)); aesop;)
+theorem LogicK.Hilbert.consistency : ⊬ᴹ(𝐊)! (⊥ : Formula α) := Logic.Hilbert.consistent α β 𝐊 trivialFrame
 
 theorem LogicKD.Hilbert.sounds (hf : Serial f) (h : ⊢ᴹ(𝐊𝐃) p) : (⊧ᴹᶠ[f] p) := Logic.Hilbert.sounds _ _ 𝐊𝐃 f ((def_FrameClass f).mp hf) h
-theorem LogicKD.Hilbert.consistency : ⊬ᴹ(𝐊𝐃)! (⊥ : Formula α) := Logic.Hilbert.consistent α β 𝐊𝐃 (by existsi ((λ _ _ => True)); aesop;)
+theorem LogicKD.Hilbert.consistency : ⊬ᴹ(𝐊𝐃)! (⊥ : Formula α) := Logic.Hilbert.consistent α β 𝐊𝐃 trivialFrame
 
--- theorem LogicS4.Hilbert.sounds (hf : Reflexive f ∧ Transitive f) (h : ⊢ᴹ(𝐒𝟒) p) : (⊧ᴹᶠ[f] p) := Logic.Hilbert.sounds _ _ 𝐒𝟒 f ((def_FrameClass f).mp hf) h
--- theorem LogicS4.Hilbert.consistency : ⊬ᴹ(𝐒𝟒)! (⊥ : Formula α) := Logic.Hilbert.consistent α β 𝐒𝟒 (by existsi ((λ _ _ => True)); aesop;)
+theorem LogicS4.Hilbert.sounds (hf : Reflexive f ∧ Transitive f) (h : ⊢ᴹ(𝐒𝟒) p) : (⊧ᴹᶠ[f] p) := Logic.Hilbert.sounds _ _ 𝐒𝟒 f ((def_FrameClass f).mp hf) h
+theorem LogicS4.Hilbert.consistency : ⊬ᴹ(𝐒𝟒)! (⊥ : Formula α) := Logic.Hilbert.consistent α β 𝐒𝟒 trivialFrame
+
+theorem LogicS5.Hilbert.sounds (hf : Reflexive f ∧ Euclidean f) (h : ⊢ᴹ(𝐒𝟓) p) : (⊧ᴹᶠ[f] p) := Logic.Hilbert.sounds _ _ 𝐒𝟓 f ((def_FrameClass f).mp hf) h
+theorem LogicS5.Hilbert.consistency : ⊬ᴹ(𝐒𝟓)! (⊥ : Formula α) := Logic.Hilbert.consistent α β 𝐒𝟓 trivialFrame
 
 end LO.Modal.Normal
